pulse/examples/steel/Duplex.PCM.fst
@@ -876,7 +876,7 @@ let rec recv_a #p c next tr =
   else (
       compatible_a_r_v_is_ahead tr tr';
       let x = next_message tr tr'.tr in
-      noop #emp ();
+      noop ();
       change_slprop
         (pts_to c (if trace_length tr >= trace_length tr'.tr then A_R next tr else extend_node_a_r tr tr'))
         (endpoint_a c (step next x) (extend tr x))
@@ -919,7 +919,7 @@ let rec recv_b #p c next tr =
   ) else (
       compatible_b_r_v_is_ahead tr tr';
       let x = next_message tr tr'.tr in
-      noop #emp ();
+      noop ();
       change_slprop
         (pts_to c (if trace_length tr >= trace_length tr'.tr then B_R next tr else extend_node_b_r tr tr'))
         (endpoint_b c (step next x) (extend tr x))
