pulse/ulib/experimental/Steel.Effect.fsti
@@ -532,10 +532,7 @@ val cond (#a:Type)
 
 val drop (p:slprop) : SteelT unit p (fun _ -> emp)
 
-val intro_exists (#a:Type) (x:a) (p:a -> slprop)
-  : SteelT unit (p x) (fun _ -> h_exists p)
-
-val noop (#[@@@ framing_implicit] p:slprop) (u:unit) : SteelT unit p (fun _ -> p)
+val noop (u:unit) : SteelT unit emp (fun _ -> emp)
 
 /// Operations on PCM Refs
 
